@prefix : <https://bimerr.iot.linkeddata.es/def/weather#> .
@prefix owl: <http://www.w3.org/2002/07/owl#> .
@prefix rdf: <http://www.w3.org/1999/02/22-rdf-syntax-ns#> .
@prefix xml: <http://www.w3.org/XML/1998/namespace> .
@prefix xsd: <http://www.w3.org/2001/XMLSchema#> .
@prefix rdfs: <http://www.w3.org/2000/01/rdf-schema#> .
@base <https://bimerr.iot.linkeddata.es/def/weather> .

<https://bimerr.iot.linkeddata.es/def/weather> rdf:type owl:Ontology ;
                                                <http://purl.org/dc/elements/1.1/decription> "Ontology for weather phenomena and exterior conditions."@en ;
                                                <http://purl.org/dc/elements/1.1/title> "BIMERR Weather Ontology"@en ;
                                                <http://purl.org/dc/terms/abstract> "Ontology for weather phenomena and exterior conditions."@en ;
                                                <http://purl.org/dc/terms/contributor> "Serge Chavez Feria https://github.com/Serge3006" ;
                                                <http://purl.org/dc/terms/creator> "Salvador Gonz√°lez Gerpe https://www.linkedin.com/in/artificialintelligence-researcher-salvadorgonzalezgerpe" ;
                                                <http://purl.org/dc/terms/license> <http://creativecommons.org/licenses/by/4.0/> ;
                                                <http://purl.org/dc/terms/publisher> <http://www.oeg-upm.net/> ;
                                                <http://purl.org/vocab/vann/preferredNamespacePrefix> "weat" ;
                                                <http://purl.org/vocab/vann/preferredNamespaceUri> "https://bimerr.iot.linkeddata.es/def/weather" .

#################################################################
#    Annotation properties
#################################################################

###  http://purl.org/dc/elements/1.1/decription
<http://purl.org/dc/elements/1.1/decription> rdf:type owl:AnnotationProperty .


###  http://purl.org/dc/elements/1.1/title
<http://purl.org/dc/elements/1.1/title> rdf:type owl:AnnotationProperty .


###  http://purl.org/dc/terms/abstract
<http://purl.org/dc/terms/abstract> rdf:type owl:AnnotationProperty .


###  http://purl.org/dc/terms/contributor
<http://purl.org/dc/terms/contributor> rdf:type owl:AnnotationProperty .


###  http://purl.org/dc/terms/creator
<http://purl.org/dc/terms/creator> rdf:type owl:AnnotationProperty .


###  http://purl.org/dc/terms/license
<http://purl.org/dc/terms/license> rdf:type owl:AnnotationProperty .


###  http://purl.org/dc/terms/publisher
<http://purl.org/dc/terms/publisher> rdf:type owl:AnnotationProperty .


###  http://purl.org/vocab/vann/preferredNamespacePrefix
<http://purl.org/vocab/vann/preferredNamespacePrefix> rdf:type owl:AnnotationProperty .


###  http://purl.org/vocab/vann/preferredNamespaceUri
<http://purl.org/vocab/vann/preferredNamespaceUri> rdf:type owl:AnnotationProperty .


###  http://schema.org/domainIncludes
<http://schema.org/domainIncludes> rdf:type owl:AnnotationProperty .


###  http://www.w3.org/2004/02/skos/core#definition
<http://www.w3.org/2004/02/skos/core#definition> rdf:type owl:AnnotationProperty .


###  http://www.w3.org/2004/02/skos/core#example
<http://www.w3.org/2004/02/skos/core#example> rdf:type owl:AnnotationProperty .


###  http://www.w3.org/2004/02/skos/core#note
<http://www.w3.org/2004/02/skos/core#note> rdf:type owl:AnnotationProperty .


#################################################################
#    Object Properties
#################################################################

###  http://www.w3.org/2003/01/geo/wgs84_pos#location
<http://www.w3.org/2003/01/geo/wgs84_pos#location> rdf:type owl:ObjectProperty ;
                                                   rdfs:subPropertyOf owl:topObjectProperty ;
                                                   rdfs:range <http://www.w3.org/2003/01/geo/wgs84_pos#SpatialThing> ;
                                                   rdfs:comment """The relation between something and the point, 
 or other geometrical thing in space, where it is.  For example, the realtionship between
 a radio tower and a Point with a given lat and long.
 Or a relationship between a park and its outline as a closed arc of points, or a road and
 its location as a arc (a sequence of points).
 Clearly in practice there will be limit to the accuracy of any such statement, but one would expect
 an accuracy appropriate for the size of the object and uses such as mapping ."""@en ;
                                                   rdfs:isDefinedBy <http://www.w3.org/2003/01/geo/wgs84_pos#> ;
                                                   rdfs:label "location"@en .


###  https://bimerr.iot.linkeddata.es/def/weat#locatedIn
<https://bimerr.iot.linkeddata.es/def/weat#locatedIn> rdf:type owl:ObjectProperty ;
                                                      rdfs:comment "Relation between Sensor and AdministrativeArea that locates it in a City and a Country."@en ;
                                                      rdfs:label "located in"@en .


###  https://saref.etsi.org/core/controlsProperty
<https://saref.etsi.org/core/controlsProperty> rdf:type owl:ObjectProperty ;
                                               rdfs:comment "A relationship specifying the property that can be controlled by a certain device"@en ;
                                               rdfs:isDefinedBy <https://saref.etsi.org/core/> ;
                                               rdfs:label "controls property"@en .


###  https://saref.etsi.org/core/hasMeasurement
<https://saref.etsi.org/core/hasMeasurement> rdf:type owl:ObjectProperty ;
                                             rdfs:comment "A relationship between a feature of interest and a measurement about it"@en ;
                                             rdfs:isDefinedBy <https://saref.etsi.org/core/> ;
                                             rdfs:label "has measurement"@en .


###  https://saref.etsi.org/core/hasProperty
<https://saref.etsi.org/core/hasProperty> rdf:type owl:ObjectProperty ;
                                          rdfs:subPropertyOf owl:topObjectProperty ;
                                          rdfs:comment "A relationship between a feature of interest and a property of that feature"@en ;
                                          rdfs:isDefinedBy <http://www.w3.org/ns/ssn/> ;
                                          rdfs:label "has property"@en .


###  https://saref.etsi.org/core/isControlledByDevice
<https://saref.etsi.org/core/isControlledByDevice> rdf:type owl:ObjectProperty ;
                                                   rdfs:comment "A relationship specifying the devices that can control a certain property"@en ;
                                                   rdfs:isDefinedBy <https://saref.etsi.org/core/> ;
                                                   rdfs:label "is controlled by device"@en .


###  https://saref.etsi.org/core/isMeasuredByDevice
<https://saref.etsi.org/core/isMeasuredByDevice> rdf:type owl:ObjectProperty ;
                                                 rdfs:comment "A relationship specifying the devices that can measure a certain property"@en ;
                                                 rdfs:isDefinedBy <https://saref.etsi.org/core/> ;
                                                 rdfs:label "is measured by device"@en .


###  https://saref.etsi.org/core/isMeasuredIn
<https://saref.etsi.org/core/isMeasuredIn> rdf:type owl:ObjectProperty ;
                                           rdfs:comment "A relationship identifying the unit of measure used for a certain entity."@en ;
                                           rdfs:isDefinedBy <https://saref.etsi.org/core/> ;
                                           rdfs:label "is measured in"@en .


###  https://saref.etsi.org/core/isMeasurementOf
<https://saref.etsi.org/core/isMeasurementOf> rdf:type owl:ObjectProperty ;
                                              rdfs:comment "A relationship between a measurement and the feature of interest whose quality was measured"@en ;
                                              rdfs:isDefinedBy <https://saref.etsi.org/core/> ;
                                              rdfs:label "is measurement of"@en .


###  https://saref.etsi.org/core/isPropertyOf
<https://saref.etsi.org/core/isPropertyOf> rdf:type owl:ObjectProperty ;
                                           rdfs:comment "A relationship between a property and the feature of interest it belongs to"@en ;
                                           rdfs:isDefinedBy <https://saref.etsi.org/core/> ;
                                           rdfs:label "is property of"@en .


###  https://saref.etsi.org/core/makeMeasurement
<https://saref.etsi.org/core/makeMeasurement> rdf:type owl:ObjectProperty ;
                                              rdfs:comment "A relation between a device and the measurements it makes. Such measurement will link together the value of the measurement, its unit of measure and the property to which it relates."@en ;
                                              rdfs:isDefinedBy <https://saref.etsi.org/core/> ;
                                              rdfs:label "make measurement"@en .


###  https://saref.etsi.org/core/measurementMadeBy
<https://saref.etsi.org/core/measurementMadeBy> rdf:type owl:ObjectProperty ;
                                                rdfs:comment "A relation between a measurement and the device that made it."@en ;
                                                rdfs:isDefinedBy <https://saref.etsi.org/core/> ;
                                                rdfs:label "measurement made by"@en .


###  https://saref.etsi.org/core/measuresProperty
<https://saref.etsi.org/core/measuresProperty> rdf:type owl:ObjectProperty ;
                                               rdfs:comment "A relationship specifying the property that can be measured by a certain device"@en ;
                                               rdfs:isDefinedBy <https://saref.etsi.org/core/> ;
                                               rdfs:label "measures property"@en .


###  https://saref.etsi.org/core/relatesToMeasurement
<https://saref.etsi.org/core/relatesToMeasurement> rdf:type owl:ObjectProperty ;
                                                   rdfs:comment "A relationship between a property and the measurements it relates to"@en ;
                                                   rdfs:isDefinedBy <https://saref.etsi.org/core/> ;
                                                   rdfs:label "relates to measurement"@en .


###  https://saref.etsi.org/core/relatesToProprety
<https://saref.etsi.org/core/relatesToProprety> rdf:type owl:ObjectProperty ;
                                                rdfs:comment "A relationship between a measurement and the property it relates to"@en ;
                                                rdfs:isDefinedBy <https://saref.etsi.org/core/> ;
                                                rdfs:label "relates to property"@en .


#################################################################
#    Data properties
#################################################################

###  http://www.w3.org/2003/01/geo/wgs84_pos#alt
<http://www.w3.org/2003/01/geo/wgs84_pos#alt> rdf:type owl:DatatypeProperty ;
                                              rdfs:comment """The WGS84 altitude of a SpatialThing (decimal meters 
above the local reference ellipsoid)."""@en ;
                                              rdfs:label "altitude"@en .


###  http://www.w3.org/2003/01/geo/wgs84_pos#lat
<http://www.w3.org/2003/01/geo/wgs84_pos#lat> rdf:type owl:DatatypeProperty ;
                                              rdfs:comment "The WGS84 latitude of a SpatialThing (decimal degrees)."@en ;
                                              rdfs:label "latitude"@en .


###  http://www.w3.org/2003/01/geo/wgs84_pos#long
<http://www.w3.org/2003/01/geo/wgs84_pos#long> rdf:type owl:DatatypeProperty ;
                                               rdfs:comment "The WGS84 longitude of a SpatialThing (decimal degrees)."@en ;
                                               rdfs:label "longitude"@en .


###  https://saref.etsi.org/core/hasTimeStamp
<https://saref.etsi.org/core/hasTimeStamp> rdf:type owl:DatatypeProperty ;
                                           rdfs:comment """Time stamp of the measure. Identify when the measurement applies to the property, which can be used either for single measurements
or for series of measurements"""@en ;
                                           rdfs:label "has time stamp"@en .


#################################################################
#    Classes
#################################################################

###  http://www.w3.org/2003/01/geo/wgs84_pos#Point
<http://www.w3.org/2003/01/geo/wgs84_pos#Point> rdf:type owl:Class ;
                                                rdfs:subClassOf <http://www.w3.org/2003/01/geo/wgs84_pos#SpatialThing> ,
                                                                [ rdf:type owl:Restriction ;
                                                                  owl:onProperty <http://www.w3.org/2003/01/geo/wgs84_pos#alt> ;
                                                                  owl:someValuesFrom xsd:decimal
                                                                ] ,
                                                                [ rdf:type owl:Restriction ;
                                                                  owl:onProperty <http://www.w3.org/2003/01/geo/wgs84_pos#lat> ;
                                                                  owl:someValuesFrom xsd:decimal
                                                                ] ,
                                                                [ rdf:type owl:Restriction ;
                                                                  owl:onProperty <http://www.w3.org/2003/01/geo/wgs84_pos#long> ;
                                                                  owl:someValuesFrom xsd:decimal
                                                                ] ;
                                                rdfs:comment "A point, typically described using a coordinate system relative to Earth, such as WGS84."@en ,
                                                             """Uniquely identified by lat/long/alt. i.e.

spaciallyIntersects(P1, P2) :- lat(P1, LAT), long(P1, LONG), alt(P1, ALT),
  lat(P2, LAT), long(P2, LONG), alt(P2, ALT).

sameThing(P1, P2) :- type(P1, Point), type(P2, Point), spaciallyIntersects(P1, P2)."""@en ;
                                                rdfs:isDefinedBy <http://www.w3.org/2003/01/geo/wgs84_pos#> ;
                                                rdfs:label "Point"@en .


###  http://www.w3.org/2003/01/geo/wgs84_pos#SpatialThing
<http://www.w3.org/2003/01/geo/wgs84_pos#SpatialThing> rdf:type owl:Class ;
                                                       rdfs:comment "Anything with spatial extent, i.e. size, shape, or position. e.g. people, places, bowling balls, as well as abstract areas like cubes."@en ;
                                                       rdfs:isDefinedBy <http://www.w3.org/2003/01/geo/wgs84_pos#> ;
                                                       rdfs:label "Spatial Thing"@en .


###  http://www.w3.org/ns/sosa/Sensor
<http://www.w3.org/ns/sosa/Sensor> rdf:type owl:Class ;
                                   rdfs:subClassOf <https://saref.etsi.org/core/Device> ;
                                   rdfs:comment "Device, agent (including humans), or software (simulation) involved in, or implementing, a Procedure. Sensors respond to a stimulus, e.g., a change in the environment, or input data composed from the results of prior Observations, and generate a Result. Sensors can be hosted by Platforms."@en ;
                                   rdfs:isDefinedBy <http://www.w3.org/ns/sosa/> ;
                                   rdfs:label "Sensor"@en ;
                                   <http://www.w3.org/2004/02/skos/core#example> "Accelerometers, gyroscopes, barometers, magnetometers, and so forth are Sensors that are typically mounted on a modern smart phone (which acts as Platform). Other examples of sensors include the human eyes."@en .


###  https://bimerr.iot.linkeddata.es/def/weat#AtmosphericPhenomenon
<https://bimerr.iot.linkeddata.es/def/weat#AtmosphericPhenomenon> rdf:type owl:Class ;
                                                                  rdfs:subClassOf <https://bimerr.iot.linkeddata.es/def/weat#WeatherProperty> ;
                                                                  rdfs:comment "A natural phenomenon involving the physical properties of matter and energy."@en ;
                                                                  rdfs:label "Atmospheric Phenomenon"@en .


###  https://bimerr.iot.linkeddata.es/def/weat#Ground
<https://bimerr.iot.linkeddata.es/def/weat#Ground> rdf:type owl:Class ;
                                                   rdfs:subClassOf <https://bimerr.iot.linkeddata.es/def/weat#WeatherProperty> ;
                                                   rdfs:comment "Ground properties where the measures are made."@en ;
                                                   rdfs:label "Ground"@en .


###  https://bimerr.iot.linkeddata.es/def/weat#Humidity
<https://bimerr.iot.linkeddata.es/def/weat#Humidity> rdf:type owl:Class ;
                                                     rdfs:subClassOf <https://bimerr.iot.linkeddata.es/def/weat#WeatherProperty> ;
                                                     rdfs:comment "Measure of the amount of moisture in the air.  It tells you how comfortable it is to be outside, and if there is enough moisture to create clouds and rain." ;
                                                     rdfs:label "Humidity"@en .


###  https://bimerr.iot.linkeddata.es/def/weat#Illuminance
<https://bimerr.iot.linkeddata.es/def/weat#Illuminance> rdf:type owl:Class ;
                                                        rdfs:subClassOf <https://bimerr.iot.linkeddata.es/def/weat#WeatherProperty> ;
                                                        rdfs:comment "The total luminous flux incident on a surface, per unit area. It is a measure of how much the incident light illuminates the surface, wavelength-weighted by the luminosity function to correlate with human brightness perception." ;
                                                        rdfs:label "Illuminance"@en .


###  https://bimerr.iot.linkeddata.es/def/weat#Precipitation
<https://bimerr.iot.linkeddata.es/def/weat#Precipitation> rdf:type owl:Class ;
                                                          rdfs:subClassOf <https://bimerr.iot.linkeddata.es/def/weat#WeatherProperty> ;
                                                          rdfs:comment "Any product of the condensation of atmospheric water vapour that falls under gravity from clouds. The main forms of precipitation include drizzle, rain, sleet, snow, ice pellets, graupel and hail." ;
                                                          rdfs:label "Precipitation"@en .


###  https://bimerr.iot.linkeddata.es/def/weat#Pressure
<https://bimerr.iot.linkeddata.es/def/weat#Pressure> rdf:type owl:Class ;
                                                     rdfs:subClassOf <https://bimerr.iot.linkeddata.es/def/weat#WeatherProperty> ;
                                                     rdfs:comment "The force exerted over a given area or object, either because of gravity pulling on it or other motion the object has.  Molecules in the air produce pressure through both their weight and movement, and this pressure is connected to other properties of the atmosphere."@en ;
                                                     rdfs:label "Pressure"@en .


###  https://bimerr.iot.linkeddata.es/def/weat#Radiation
<https://bimerr.iot.linkeddata.es/def/weat#Radiation> rdf:type owl:Class ;
                                                      rdfs:subClassOf <https://bimerr.iot.linkeddata.es/def/weat#WeatherProperty> ;
                                                      rdfs:comment "The emission or transmission of energy in the form of waves or particles through space or through a material medium."@en ;
                                                      rdfs:label "Radiation"@en .


###  https://bimerr.iot.linkeddata.es/def/weat#SkyCover
<https://bimerr.iot.linkeddata.es/def/weat#SkyCover> rdf:type owl:Class ;
                                                     rdfs:subClassOf <https://bimerr.iot.linkeddata.es/def/weat#WeatherProperty> ;
                                                     rdfs:comment "The extent to which the sky is obscured by clouds."@en ;
                                                     rdfs:label "Sky Cover"@en .


###  https://bimerr.iot.linkeddata.es/def/weat#Snow
<https://bimerr.iot.linkeddata.es/def/weat#Snow> rdf:type owl:Class ;
                                                 rdfs:subClassOf <https://bimerr.iot.linkeddata.es/def/weat#Precipitation> ;
                                                 rdfs:comment "Individual ice crystals that grow while suspended in the atmosphere‚Äîusually within clouds‚Äîand then fall, accumulating on the ground where they undergo further changes."@en ;
                                                 rdfs:label "Snow"@en .


###  https://bimerr.iot.linkeddata.es/def/weat#Storm
<https://bimerr.iot.linkeddata.es/def/weat#Storm> rdf:type owl:Class ;
                                                  rdfs:subClassOf <https://bimerr.iot.linkeddata.es/def/weat#Precipitation> ;
                                                  rdfs:comment "Any disturbed state of a body especially affecting its surface, and strongly implying a wind force. It may be marked by significant disruptions and lightning (a thunderstorm), heavy precipitation (snowstorm, rainstorm), heavy freezing rain (ice storm), strong winds (tropical cyclone, windstorm), or wind transporting some substance through the atmosphere as in a dust storm, blizzard, sandstorm, etc."@en ;
                                                  rdfs:label "Storm"@en .


###  https://bimerr.iot.linkeddata.es/def/weat#Temperature
<https://bimerr.iot.linkeddata.es/def/weat#Temperature> rdf:type owl:Class ;
                                                        rdfs:subClassOf <https://bimerr.iot.linkeddata.es/def/weat#WeatherProperty> ;
                                                        rdfs:comment "The measure of thermal or internal energy of the molecules within an object or gas.    We can measure temperature of an object using either direct contact or remote sensing.  Temperature of air is closely related to other atmospheric properties, such as pressure, volume and density."@en ;
                                                        rdfs:label "Temperature"@en .


###  https://bimerr.iot.linkeddata.es/def/weat#Time
<https://bimerr.iot.linkeddata.es/def/weat#Time> rdf:type owl:Class ;
                                                 rdfs:subClassOf <https://bimerr.iot.linkeddata.es/def/weat#WeatherProperty> ;
                                                 rdfs:comment "The indefinite continued progress of existence and events that occur in an apparently irreversible succession from the past, through the present, into the future." ;
                                                 rdfs:label "Time"@en .


###  https://bimerr.iot.linkeddata.es/def/weat#WeatherProperty
<https://bimerr.iot.linkeddata.es/def/weat#WeatherProperty> rdf:type owl:Class ;
                                                            rdfs:subClassOf <https://saref.etsi.org/core/Property> ;
                                                            rdfs:comment "Property type to classify  weather data."@en ;
                                                            rdfs:label "Weather Property"@en .


###  https://bimerr.iot.linkeddata.es/def/weat#Wind
<https://bimerr.iot.linkeddata.es/def/weat#Wind> rdf:type owl:Class ;
                                                 rdfs:subClassOf <https://bimerr.iot.linkeddata.es/def/weat#AtmosphericPhenomenon> ;
                                                 rdfs:comment "The perceptible natural movement of the air, especially in the form of a current of air blowing from a particular direction." .


###  https://saref.etsi.org/core/Device
<https://saref.etsi.org/core/Device> rdf:type owl:Class ;
                                     rdfs:subClassOf [ rdf:type owl:Restriction ;
                                                       owl:onProperty <http://www.w3.org/2003/01/geo/wgs84_pos#location> ;
                                                       owl:someValuesFrom <http://www.w3.org/2003/01/geo/wgs84_pos#SpatialThing>
                                                     ] ,
                                                     [ rdf:type owl:Restriction ;
                                                       owl:onProperty <https://bimerr.iot.linkeddata.es/def/weat#locatedIn> ;
                                                       owl:someValuesFrom <https://w3id.org/def/saref4city#AdministrativeArea>
                                                     ] ;
                                     rdfs:comment "A tangible object designed to accomplish a particular task in households, common public buildings or offices. In order to accomplish this task, the device performs one or more functions. For example, a washing machine is designed to wash (task) and to accomplish this task it performs a start and stop function."@en ;
                                     rdfs:isDefinedBy <https://saref.etsi.org/core/> ;
                                     rdfs:label "Device"@en .


###  https://saref.etsi.org/core/FeatureOfInterest
<https://saref.etsi.org/core/FeatureOfInterest> rdf:type owl:Class ;
                                                rdfs:subClassOf [ rdf:type owl:Restriction ;
                                                                  owl:onProperty <https://saref.etsi.org/core/hasMeasurement> ;
                                                                  owl:someValuesFrom <https://saref.etsi.org/core/Measurement>
                                                                ] ,
                                                                [ rdf:type owl:Restriction ;
                                                                  owl:onProperty <https://saref.etsi.org/core/hasProperty> ;
                                                                  owl:someValuesFrom <https://saref.etsi.org/core/Property>
                                                                ] ,
                                                                [ rdf:type owl:Restriction ;
                                                                  owl:onProperty <https://saref.etsi.org/core/hasProperty> ;
                                                                  owl:minCardinality "1"^^xsd:nonNegativeInteger
                                                                ] ;
                                                rdfs:comment "A feature of interest represents any real world entity from which a property is measured. It is linked to the different properties it has and to its measurements."@en ;
                                                rdfs:isDefinedBy <https://saref.etsi.org/core/> ;
                                                rdfs:label "Feature of Interest"@en ;
                                                <http://www.w3.org/2004/02/skos/core#example> "When measuring the height of a tree, the height is the observed ObservableProperty, 20m may be the Result of the Observation, and the tree is the FeatureOfInterest. A window is a FeatureOfInterest for an automatic window control Actuator."@en .


###  https://saref.etsi.org/core/Measurement
<https://saref.etsi.org/core/Measurement> rdf:type owl:Class ;
                                          rdfs:subClassOf [ rdf:type owl:Restriction ;
                                                            owl:onProperty <https://saref.etsi.org/core/isMeasuredIn> ;
                                                            owl:someValuesFrom <https://w3id.org/saref#UnitOfMeasure>
                                                          ] ,
                                                          [ rdf:type owl:Restriction ;
                                                            owl:onProperty <https://saref.etsi.org/core/isMeasurementOf> ;
                                                            owl:someValuesFrom <https://saref.etsi.org/core/FeatureOfInterest>
                                                          ] ,
                                                          [ rdf:type owl:Restriction ;
                                                            owl:onProperty <https://saref.etsi.org/core/measurementMadeBy> ;
                                                            owl:someValuesFrom <https://saref.etsi.org/core/Device>
                                                          ] ,
                                                          [ rdf:type owl:Restriction ;
                                                            owl:onProperty <https://saref.etsi.org/core/relatesToProprety> ;
                                                            owl:someValuesFrom <https://saref.etsi.org/core/Property>
                                                          ] ,
                                                          [ rdf:type owl:Restriction ;
                                                            owl:onProperty <https://saref.etsi.org/core/hasTimeStamp> ;
                                                            owl:someValuesFrom xsd:dateTime
                                                          ] ;
                                          rdfs:comment "The measured value made over a property. It is also linked to the unit of measure in which the value is expressed and to the timestamp of the measurement."@en ;
                                          rdfs:isDefinedBy <https://saref.etsi.org/core/> ;
                                          rdfs:label "Measurement"@en .


###  https://saref.etsi.org/core/Property
<https://saref.etsi.org/core/Property> rdf:type owl:Class ;
                                       rdfs:subClassOf [ rdf:type owl:Restriction ;
                                                         owl:onProperty <https://saref.etsi.org/core/isControlledByDevice> ;
                                                         owl:someValuesFrom <https://saref.etsi.org/core/Device>
                                                       ] ,
                                                       [ rdf:type owl:Restriction ;
                                                         owl:onProperty <https://saref.etsi.org/core/isMeasuredByDevice> ;
                                                         owl:someValuesFrom <https://saref.etsi.org/core/Device>
                                                       ] ,
                                                       [ rdf:type owl:Restriction ;
                                                         owl:onProperty <https://saref.etsi.org/core/isPropertyOf> ;
                                                         owl:someValuesFrom <https://saref.etsi.org/core/FeatureOfInterest>
                                                       ] ,
                                                       [ rdf:type owl:Restriction ;
                                                         owl:onProperty <https://saref.etsi.org/core/relatesToMeasurement> ;
                                                         owl:someValuesFrom <https://saref.etsi.org/core/Measurement>
                                                       ] ;
                                       rdfs:comment "Anything that can be sensed, measured or controlled in households, common public buildings or offices. A list of properties that are relevant for the purpose of SAREF is proposed, but this list can be extended."@en ;
                                       rdfs:isDefinedBy <http://www.w3.org/ns/ssn/> ;
                                       rdfs:label "Property"@en .


###  https://w3id.org/def/saref4city#AdministrativeArea
<https://w3id.org/def/saref4city#AdministrativeArea> rdf:type owl:Class ;
                                                     rdfs:comment "An administrative division, unit, entity, area or region, also referred to as a subnational entity, constituent unit, or country subdivision, is a portion of a country or other region delineated for the purpose of administration. (https://en.wikipedia.org/wiki/Administrative_division)"@en ;
                                                     rdfs:isDefinedBy <https://w3id.org/def/saref4city#> ;
                                                     rdfs:label "Administrative Area"@en .


###  https://w3id.org/def/saref4city#City
<https://w3id.org/def/saref4city#City> rdf:type owl:Class ;
                                       rdfs:subClassOf <https://w3id.org/def/saref4city#AdministrativeArea> ;
                                       rdfs:comment "A city is a large human settlement. A city is distinguished from other human settlements by its relatively great size, but also by its functions and its special symbolic status, which may be conferred by a central authority. (https://en.wikipedia.org/wiki/City)"@en ;
                                       rdfs:isDefinedBy <https://w3id.org/def/saref4city#> ;
                                       rdfs:label "City"@en .


###  https://w3id.org/def/saref4city#Country
<https://w3id.org/def/saref4city#Country> rdf:type owl:Class ;
                                          rdfs:subClassOf <https://w3id.org/def/saref4city#AdministrativeArea> ;
                                          rdfs:comment "A country is a region that is identified as a distinct national entity in political geography. (https://en.wikipedia.org/wiki/Country)"@en ;
                                          rdfs:isDefinedBy <https://w3id.org/def/saref4city#> ;
                                          rdfs:label "Country"@en .


###  https://w3id.org/saref#UnitOfMeasure
<https://w3id.org/saref#UnitOfMeasure> rdf:type owl:Class ;
                                       rdfs:comment "The unit of measure is a standard for measurement of a quantity, such as a saref:Property. For example, Power is a property and Watt is a unit of power that represents a definite predetermined power: when it is said 10 Watt, it is actually meant 10 times the definite predetermined power called \"watt\". The definition of unit of measure in SAREF refers to the definition of unit of measure in the Ontology of units of Measure (OM). A list of some units of measure that are relevant for the purpose of SAREF is proposed, but this list can be extended, also using some other ontologies rather than the Ontology of units of Measure (OM)."@en ;
                                       rdfs:isDefinedBy <https://w3id.org/saref#> ;
                                       rdfs:label "Unit of Measure"@en .


#################################################################
#    Individuals
#################################################################

###  http://www.ontology-of-units-of-measure.org/resource/om-2/Density
<http://www.ontology-of-units-of-measure.org/resource/om-2/Density> rdf:type owl:NamedIndividual ,
                                                                             <https://w3id.org/saref#UnitOfMeasure> .


###  http://www.ontology-of-units-of-measure.org/resource/om-2/candelaPerSquareMetre
<http://www.ontology-of-units-of-measure.org/resource/om-2/candelaPerSquareMetre> rdf:type owl:NamedIndividual ,
                                                                                           <https://w3id.org/saref#UnitOfMeasure> .


###  http://www.ontology-of-units-of-measure.org/resource/om-2/centimetre
<http://www.ontology-of-units-of-measure.org/resource/om-2/centimetre> rdf:type owl:NamedIndividual ,
                                                                                <https://w3id.org/saref#UnitOfMeasure> .


###  http://www.ontology-of-units-of-measure.org/resource/om-2/day
<http://www.ontology-of-units-of-measure.org/resource/om-2/day> rdf:type owl:NamedIndividual ,
                                                                         <https://w3id.org/saref#UnitOfMeasure> .


###  http://www.ontology-of-units-of-measure.org/resource/om-2/degree
<http://www.ontology-of-units-of-measure.org/resource/om-2/degree> rdf:type owl:NamedIndividual ,
                                                                            <https://w3id.org/saref#UnitOfMeasure> .


###  http://www.ontology-of-units-of-measure.org/resource/om-2/degreeCelsius
<http://www.ontology-of-units-of-measure.org/resource/om-2/degreeCelsius> rdf:type owl:NamedIndividual ,
                                                                                   <https://w3id.org/saref#UnitOfMeasure> .


###  http://www.ontology-of-units-of-measure.org/resource/om-2/degreeFahrenheit
<http://www.ontology-of-units-of-measure.org/resource/om-2/degreeFahrenheit> rdf:type owl:NamedIndividual ,
                                                                                      <https://w3id.org/saref#UnitOfMeasure> .


###  http://www.ontology-of-units-of-measure.org/resource/om-2/hour
<http://www.ontology-of-units-of-measure.org/resource/om-2/hour> rdf:type owl:NamedIndividual ,
                                                                          <https://w3id.org/saref#UnitOfMeasure> .


###  http://www.ontology-of-units-of-measure.org/resource/om-2/inch-International
<http://www.ontology-of-units-of-measure.org/resource/om-2/inch-International> rdf:type owl:NamedIndividual ,
                                                                                        <https://w3id.org/saref#UnitOfMeasure> .


###  http://www.ontology-of-units-of-measure.org/resource/om-2/joulePerKilogram
<http://www.ontology-of-units-of-measure.org/resource/om-2/joulePerKilogram> rdf:type owl:NamedIndividual ,
                                                                                      <https://w3id.org/saref#UnitOfMeasure> .


###  http://www.ontology-of-units-of-measure.org/resource/om-2/kilogramPerCubicmetre
<http://www.ontology-of-units-of-measure.org/resource/om-2/kilogramPerCubicmetre> rdf:type owl:NamedIndividual ,
                                                                                           <https://w3id.org/saref#UnitOfMeasure> .


###  http://www.ontology-of-units-of-measure.org/resource/om-2/kilometre
<http://www.ontology-of-units-of-measure.org/resource/om-2/kilometre> rdf:type owl:NamedIndividual ,
                                                                               <https://w3id.org/saref#UnitOfMeasure> .


###  http://www.ontology-of-units-of-measure.org/resource/om-2/lux
<http://www.ontology-of-units-of-measure.org/resource/om-2/lux> rdf:type owl:NamedIndividual ,
                                                                         <https://w3id.org/saref#UnitOfMeasure> .


###  http://www.ontology-of-units-of-measure.org/resource/om-2/metre
<http://www.ontology-of-units-of-measure.org/resource/om-2/metre> rdf:type owl:NamedIndividual ,
                                                                           <https://w3id.org/saref#UnitOfMeasure> .


###  http://www.ontology-of-units-of-measure.org/resource/om-2/metrePerSecond-Time
<http://www.ontology-of-units-of-measure.org/resource/om-2/metrePerSecond-Time> rdf:type owl:NamedIndividual ,
                                                                                         <https://w3id.org/saref#UnitOfMeasure> .


###  http://www.ontology-of-units-of-measure.org/resource/om-2/mile-Statute
<http://www.ontology-of-units-of-measure.org/resource/om-2/mile-Statute> rdf:type owl:NamedIndividual ,
                                                                                  <https://w3id.org/saref#UnitOfMeasure> .


###  http://www.ontology-of-units-of-measure.org/resource/om-2/mile-StatutePerHour
<http://www.ontology-of-units-of-measure.org/resource/om-2/mile-StatutePerHour> rdf:type owl:NamedIndividual ,
                                                                                         <https://w3id.org/saref#UnitOfMeasure> .


###  http://www.ontology-of-units-of-measure.org/resource/om-2/millibar
<http://www.ontology-of-units-of-measure.org/resource/om-2/millibar> rdf:type owl:NamedIndividual ,
                                                                              <https://w3id.org/saref#UnitOfMeasure> .


###  http://www.ontology-of-units-of-measure.org/resource/om-2/millimetre
<http://www.ontology-of-units-of-measure.org/resource/om-2/millimetre> rdf:type owl:NamedIndividual ,
                                                                                <https://w3id.org/saref#UnitOfMeasure> .


###  http://www.ontology-of-units-of-measure.org/resource/om-2/pascal
<http://www.ontology-of-units-of-measure.org/resource/om-2/pascal> rdf:type owl:NamedIndividual ,
                                                                            <https://w3id.org/saref#UnitOfMeasure> .


###  http://www.ontology-of-units-of-measure.org/resource/om-2/percent
<http://www.ontology-of-units-of-measure.org/resource/om-2/percent> rdf:type owl:NamedIndividual ,
                                                                             <https://w3id.org/saref#UnitOfMeasure> .


###  http://www.ontology-of-units-of-measure.org/resource/om-2/wattPerMetreKelvin
<http://www.ontology-of-units-of-measure.org/resource/om-2/wattPerMetreKelvin> rdf:type owl:NamedIndividual ,
                                                                                        <https://w3id.org/saref#UnitOfMeasure> .


###  https://bimerr.iot.linkeddata.es/def/weat#AerosolOpticalDepth
<https://bimerr.iot.linkeddata.es/def/weat#AerosolOpticalDepth> rdf:type owl:NamedIndividual ,
                                                                         <https://bimerr.iot.linkeddata.es/def/weat#Radiation> ;
                                                                rdfs:comment "An individual representing the radiation property aerosol optical depth from EPW." .


###  https://bimerr.iot.linkeddata.es/def/weat#Albedo
<https://bimerr.iot.linkeddata.es/def/weat#Albedo> rdf:type owl:NamedIndividual ,
                                                            <https://bimerr.iot.linkeddata.es/def/weat#Radiation> ;
                                                   rdfs:comment "An individual representing the radiation property albedo from EPW." .


###  https://bimerr.iot.linkeddata.es/def/weat#AtmosphericStationPressure
<https://bimerr.iot.linkeddata.es/def/weat#AtmosphericStationPressure> rdf:type owl:NamedIndividual ,
                                                                                <https://bimerr.iot.linkeddata.es/def/weat#Pressure> ;
                                                                       rdfs:comment "An individual representing the pressure property atmospheric station pressure." .


###  https://bimerr.iot.linkeddata.es/def/weat#AverageTemperatureForPeriod
<https://bimerr.iot.linkeddata.es/def/weat#AverageTemperatureForPeriod> rdf:type owl:NamedIndividual ,
                                                                                 <https://bimerr.iot.linkeddata.es/def/weat#Temperature> ;
                                                                        rdfs:comment "An individual representing the average temperature for period from EPW."@en .


###  https://bimerr.iot.linkeddata.es/def/weat#CeillingHeight
<https://bimerr.iot.linkeddata.es/def/weat#CeillingHeight> rdf:type owl:NamedIndividual ,
                                                                    <https://bimerr.iot.linkeddata.es/def/weat#WeatherProperty> ;
                                                           rdfs:comment "An individual representing the weather property ceilling height." .


###  https://bimerr.iot.linkeddata.es/def/weat#DataSourceAndUncertaintyFlags
<https://bimerr.iot.linkeddata.es/def/weat#DataSourceAndUncertaintyFlags> rdf:type owl:NamedIndividual ,
                                                                                   <https://bimerr.iot.linkeddata.es/def/weat#WeatherProperty> ;
                                                                          rdfs:comment "An individual representing the weather property data source and uncertainty flags." .


###  https://bimerr.iot.linkeddata.es/def/weat#DaysSinceLastSnowfall
<https://bimerr.iot.linkeddata.es/def/weat#DaysSinceLastSnowfall> rdf:type owl:NamedIndividual ,
                                                                           <https://bimerr.iot.linkeddata.es/def/weat#Snow> ;
                                                                  rdfs:comment "An individual representing the snow property days since last snowfall time from EPW." .


###  https://bimerr.iot.linkeddata.es/def/weat#DewPointTemperature
<https://bimerr.iot.linkeddata.es/def/weat#DewPointTemperature> rdf:type owl:NamedIndividual ,
                                                                         <https://bimerr.iot.linkeddata.es/def/weat#Temperature> ;
                                                                rdfs:comment "An individual representing the temperature property dew point temperature from EPW and Dark Sky API, first measured in Celsius degrees and second in Fahrenheit degrees." .


###  https://bimerr.iot.linkeddata.es/def/weat#DiffuseHorizontalRadiation
<https://bimerr.iot.linkeddata.es/def/weat#DiffuseHorizontalRadiation> rdf:type owl:NamedIndividual ,
                                                                                <https://bimerr.iot.linkeddata.es/def/weat#Radiation> ;
                                                                       rdfs:comment "An individual representing the radiation property diffuse horizontal radiation from EPW." .


###  https://bimerr.iot.linkeddata.es/def/weat#DirectHorizontalIlluminance
<https://bimerr.iot.linkeddata.es/def/weat#DirectHorizontalIlluminance> rdf:type owl:NamedIndividual ,
                                                                                 <https://bimerr.iot.linkeddata.es/def/weat#Illuminance> ;
                                                                        rdfs:comment "An individual representing the illuminance property direct horizontal illuminance from EPW." .


###  https://bimerr.iot.linkeddata.es/def/weat#DirectNormalIlluminance
<https://bimerr.iot.linkeddata.es/def/weat#DirectNormalIlluminance> rdf:type owl:NamedIndividual ,
                                                                             <https://bimerr.iot.linkeddata.es/def/weat#Illuminance> ;
                                                                    rdfs:comment "An individual representing the illuminance property direct normal illuminance from EPW." .


###  https://bimerr.iot.linkeddata.es/def/weat#DirectNormalRadiation
<https://bimerr.iot.linkeddata.es/def/weat#DirectNormalRadiation> rdf:type owl:NamedIndividual ,
                                                                           <https://bimerr.iot.linkeddata.es/def/weat#Radiation> ;
                                                                  rdfs:comment "An individual representing the radiation property direct normal radiation from EPW." .


###  https://bimerr.iot.linkeddata.es/def/weat#DryBulbTemperature
<https://bimerr.iot.linkeddata.es/def/weat#DryBulbTemperature> rdf:type owl:NamedIndividual ,
                                                                        <https://bimerr.iot.linkeddata.es/def/weat#Temperature> ;
                                                               rdfs:comment "An individual representing the temperature property dry bulb temperature from EPW." .


###  https://bimerr.iot.linkeddata.es/def/weat#ExtraterrestialDirectNormalRadiation
<https://bimerr.iot.linkeddata.es/def/weat#ExtraterrestialDirectNormalRadiation> rdf:type owl:NamedIndividual ,
                                                                                          <https://bimerr.iot.linkeddata.es/def/weat#Radiation> ;
                                                                                 rdfs:comment "An individual representing the radiation property extraterrestial direct normal radiation from EPW." .


###  https://bimerr.iot.linkeddata.es/def/weat#ExtraterrestialHorizontalRadiation
<https://bimerr.iot.linkeddata.es/def/weat#ExtraterrestialHorizontalRadiation> rdf:type owl:NamedIndividual ,
                                                                                        <https://bimerr.iot.linkeddata.es/def/weat#Radiation> ;
                                                                               rdfs:comment "An individual representing the radiation property extrzaterrestial horizontal radiation from EPW." .


###  https://bimerr.iot.linkeddata.es/def/weat#GlobalHorizontalIlluminance
<https://bimerr.iot.linkeddata.es/def/weat#GlobalHorizontalIlluminance> rdf:type owl:NamedIndividual ,
                                                                                 <https://bimerr.iot.linkeddata.es/def/weat#Illuminance> ;
                                                                        rdfs:comment "An individual representing the illuminance property global horizontal illuminance from EPW." .


###  https://bimerr.iot.linkeddata.es/def/weat#GlobalHorizontalRadiation
<https://bimerr.iot.linkeddata.es/def/weat#GlobalHorizontalRadiation> rdf:type owl:NamedIndividual ,
                                                                               <https://bimerr.iot.linkeddata.es/def/weat#Radiation> ;
                                                                      rdfs:comment "An individual representing the radiation property global horizontal radiation from EPW." .


###  https://bimerr.iot.linkeddata.es/def/weat#GroundConductivity
<https://bimerr.iot.linkeddata.es/def/weat#GroundConductivity> rdf:type owl:NamedIndividual ,
                                                                        <https://bimerr.iot.linkeddata.es/def/weat#Ground> ;
                                                               rdfs:comment "An individual representing the ground conductivity from EPW."@en .


###  https://bimerr.iot.linkeddata.es/def/weat#GroundDensity
<https://bimerr.iot.linkeddata.es/def/weat#GroundDensity> rdf:type owl:NamedIndividual ,
                                                                   <https://bimerr.iot.linkeddata.es/def/weat#Ground> ;
                                                          rdfs:comment "An individual representing the ground density from EPW."@en .


###  https://bimerr.iot.linkeddata.es/def/weat#GroundSpecificHeat
<https://bimerr.iot.linkeddata.es/def/weat#GroundSpecificHeat> rdf:type owl:NamedIndividual ,
                                                                        <https://bimerr.iot.linkeddata.es/def/weat#Ground> ;
                                                               rdfs:comment "An individual representing the ground specific heat from EPW."@en .


###  https://bimerr.iot.linkeddata.es/def/weat#GroundTemperature
<https://bimerr.iot.linkeddata.es/def/weat#GroundTemperature> rdf:type owl:NamedIndividual ,
                                                                       <https://bimerr.iot.linkeddata.es/def/weat#Ground> ;
                                                              rdfs:comment "An individual representing the ground temperature from EPW."@en .


###  https://bimerr.iot.linkeddata.es/def/weat#GroundTemperatureDepth
<https://bimerr.iot.linkeddata.es/def/weat#GroundTemperatureDepth> rdf:type owl:NamedIndividual ,
                                                                            <https://bimerr.iot.linkeddata.es/def/weat#Ground> ;
                                                                   rdfs:comment "An individual representing the ground temperature depth from EPW."@en .


###  https://bimerr.iot.linkeddata.es/def/weat#HorizontalInfraredRadiationIntensity
<https://bimerr.iot.linkeddata.es/def/weat#HorizontalInfraredRadiationIntensity> rdf:type owl:NamedIndividual ,
                                                                                          <https://bimerr.iot.linkeddata.es/def/weat#Radiation> ;
                                                                                 rdfs:comment "An individual representing the radiation property horizontal infrared radiation instensity from EPW." .


###  https://bimerr.iot.linkeddata.es/def/weat#InchesPerHour
<https://bimerr.iot.linkeddata.es/def/weat#InchesPerHour> rdf:type owl:NamedIndividual ,
                                                                   <https://w3id.org/saref#UnitOfMeasure> .


###  https://bimerr.iot.linkeddata.es/def/weat#LiquidPrecipitationDepth
<https://bimerr.iot.linkeddata.es/def/weat#LiquidPrecipitationDepth> rdf:type owl:NamedIndividual ,
                                                                              <https://bimerr.iot.linkeddata.es/def/weat#Precipitation> ;
                                                                     rdfs:comment "An individual representing the precipitation property liquid precipitation depth from EPW." .


###  https://bimerr.iot.linkeddata.es/def/weat#LiquidPrecipitationQuantity
<https://bimerr.iot.linkeddata.es/def/weat#LiquidPrecipitationQuantity> rdf:type owl:NamedIndividual ,
                                                                                 <https://bimerr.iot.linkeddata.es/def/weat#Precipitation> ;
                                                                        rdfs:comment "An individual representing the precipitation property liquid precipitation quantity from EPW." .


###  https://bimerr.iot.linkeddata.es/def/weat#MaxTemperatureForPeriod
<https://bimerr.iot.linkeddata.es/def/weat#MaxTemperatureForPeriod> rdf:type owl:NamedIndividual ,
                                                                             <https://bimerr.iot.linkeddata.es/def/weat#Temperature> ;
                                                                    rdfs:comment "An individual representing the max temperature for period from EPW."@en .


###  https://bimerr.iot.linkeddata.es/def/weat#MinTemperatureForPeriod
<https://bimerr.iot.linkeddata.es/def/weat#MinTemperatureForPeriod> rdf:type owl:NamedIndividual ,
                                                                             <https://bimerr.iot.linkeddata.es/def/weat#Temperature> ;
                                                                    rdfs:comment "An individual representing the min temperature for period from EPW."@en .


###  https://bimerr.iot.linkeddata.es/def/weat#OpaqueSkycover
<https://bimerr.iot.linkeddata.es/def/weat#OpaqueSkycover> rdf:type owl:NamedIndividual ,
                                                                    <https://bimerr.iot.linkeddata.es/def/weat#SkyCover> ;
                                                           rdfs:comment "An individual representing the sky cover property opaque sky cover from EPW." .


###  https://bimerr.iot.linkeddata.es/def/weat#Period
<https://bimerr.iot.linkeddata.es/def/weat#Period> rdf:type owl:NamedIndividual ,
                                                            <https://bimerr.iot.linkeddata.es/def/weat#Time> ;
                                                   rdfs:comment "An individual representing the preiod for the max, min and average temperature periods from EPW."@en .


###  https://bimerr.iot.linkeddata.es/def/weat#PrecipitableWater
<https://bimerr.iot.linkeddata.es/def/weat#PrecipitableWater> rdf:type owl:NamedIndividual ,
                                                                       <https://bimerr.iot.linkeddata.es/def/weat#Precipitation> ;
                                                              rdfs:comment "An individual representing the precipitation property precipitable water from EPW." .


###  https://bimerr.iot.linkeddata.es/def/weat#PresentWeatherCodes
<https://bimerr.iot.linkeddata.es/def/weat#PresentWeatherCodes> rdf:type owl:NamedIndividual ,
                                                                         <https://bimerr.iot.linkeddata.es/def/weat#WeatherProperty> ;
                                                                rdfs:comment "An individual representing the weather property present weather codes from EPW." .


###  https://bimerr.iot.linkeddata.es/def/weat#PresentWeatherObservation
<https://bimerr.iot.linkeddata.es/def/weat#PresentWeatherObservation> rdf:type owl:NamedIndividual ,
                                                                               <https://bimerr.iot.linkeddata.es/def/weat#WeatherProperty> .


###  https://bimerr.iot.linkeddata.es/def/weat#RelativeHumidity
<https://bimerr.iot.linkeddata.es/def/weat#RelativeHumidity> rdf:type owl:NamedIndividual ,
                                                                      <https://bimerr.iot.linkeddata.es/def/weat#Humidity> ;
                                                             rdfs:comment "An individual representing the humidity property relative humidity from EPW." .


###  https://bimerr.iot.linkeddata.es/def/weat#SnowDepth
<https://bimerr.iot.linkeddata.es/def/weat#SnowDepth> rdf:type owl:NamedIndividual ,
                                                               <https://bimerr.iot.linkeddata.es/def/weat#Snow> ;
                                                      rdfs:comment "An individual representing the snow property snow depth from EPW." .


###  https://bimerr.iot.linkeddata.es/def/weat#TenthsOfCoverage
<https://bimerr.iot.linkeddata.es/def/weat#TenthsOfCoverage> rdf:type owl:NamedIndividual ,
                                                                      <https://w3id.org/saref#UnitOfMeasure> .


###  https://bimerr.iot.linkeddata.es/def/weat#Thousandths
<https://bimerr.iot.linkeddata.es/def/weat#Thousandths> rdf:type owl:NamedIndividual ,
                                                                 <https://w3id.org/saref#UnitOfMeasure> .


###  https://bimerr.iot.linkeddata.es/def/weat#TotalSkyCover
<https://bimerr.iot.linkeddata.es/def/weat#TotalSkyCover> rdf:type owl:NamedIndividual ,
                                                                   <https://bimerr.iot.linkeddata.es/def/weat#SkyCover> ;
                                                          rdfs:comment "An individual representing the sky cover property total sky cover from EPW." .


###  https://bimerr.iot.linkeddata.es/def/weat#Visibility
<https://bimerr.iot.linkeddata.es/def/weat#Visibility> rdf:type owl:NamedIndividual ,
                                                                <https://bimerr.iot.linkeddata.es/def/weat#WeatherProperty> ;
                                                       rdfs:comment "An individual representing the weather property visibility from EPW." .


###  https://bimerr.iot.linkeddata.es/def/weat#WattHourPerSquareMetre
<https://bimerr.iot.linkeddata.es/def/weat#WattHourPerSquareMetre> rdf:type owl:NamedIndividual ,
                                                                            <https://w3id.org/saref#UnitOfMeasure> .


###  https://bimerr.iot.linkeddata.es/def/weat#WindDirection
<https://bimerr.iot.linkeddata.es/def/weat#WindDirection> rdf:type owl:NamedIndividual ,
                                                                   <https://bimerr.iot.linkeddata.es/def/weat#Wind> ;
                                                          rdfs:comment "An individual representing the wind property wind direction from EPW." .


###  https://bimerr.iot.linkeddata.es/def/weat#ZenithLuminance
<https://bimerr.iot.linkeddata.es/def/weat#ZenithLuminance> rdf:type owl:NamedIndividual ,
                                                                     <https://bimerr.iot.linkeddata.es/def/weat#Illuminance> ;
                                                            rdfs:comment "An individual representing the illuminance property zenith luminance from EPW." .


###  https://bimerr.iot.linkeddata.es/def/weat#apparentTemperature
<https://bimerr.iot.linkeddata.es/def/weat#apparentTemperature> rdf:type owl:NamedIndividual ,
                                                                         <https://bimerr.iot.linkeddata.es/def/weat#Temperature> ;
                                                                rdfs:comment "An individual representing the temperature property apparent temperature from Dark Sky API." .


###  https://bimerr.iot.linkeddata.es/def/weat#apparentTemperatureHigh
<https://bimerr.iot.linkeddata.es/def/weat#apparentTemperatureHigh> rdf:type owl:NamedIndividual ,
                                                                             <https://bimerr.iot.linkeddata.es/def/weat#Temperature> ;
                                                                    rdfs:comment "An individual representing the temperature property apparent temperature high from Dark Sky API." .


###  https://bimerr.iot.linkeddata.es/def/weat#apparentTemperatureHighTime
<https://bimerr.iot.linkeddata.es/def/weat#apparentTemperatureHighTime> rdf:type owl:NamedIndividual ,
                                                                                 <https://bimerr.iot.linkeddata.es/def/weat#Time> ;
                                                                        rdfs:comment "An individual representing the time property apparent temperature high time from Dark Sky API." .


###  https://bimerr.iot.linkeddata.es/def/weat#apparentTemperatureLow
<https://bimerr.iot.linkeddata.es/def/weat#apparentTemperatureLow> rdf:type owl:NamedIndividual ,
                                                                            <https://bimerr.iot.linkeddata.es/def/weat#Temperature> ;
                                                                   rdfs:comment "An individual representing the temperature property apparent temperature low from Dark Sky API." .


###  https://bimerr.iot.linkeddata.es/def/weat#apparentTemperatureLowTime
<https://bimerr.iot.linkeddata.es/def/weat#apparentTemperatureLowTime> rdf:type owl:NamedIndividual ,
                                                                                <https://bimerr.iot.linkeddata.es/def/weat#Time> ;
                                                                       rdfs:comment "An individual representing the time property apparent temperature low time from Dark Sky API." .


###  https://bimerr.iot.linkeddata.es/def/weat#apparentTemperatureMax
<https://bimerr.iot.linkeddata.es/def/weat#apparentTemperatureMax> rdf:type owl:NamedIndividual ,
                                                                            <https://bimerr.iot.linkeddata.es/def/weat#Temperature> ;
                                                                   rdfs:comment "An individual representing the temperature property apparent temperature max from Dark Sky API." .


###  https://bimerr.iot.linkeddata.es/def/weat#apparentTemperatureMaxTime
<https://bimerr.iot.linkeddata.es/def/weat#apparentTemperatureMaxTime> rdf:type owl:NamedIndividual ,
                                                                                <https://bimerr.iot.linkeddata.es/def/weat#Time> ;
                                                                       rdfs:comment "An individual representing the time property apparent temperature max time from Dark Sky API." .


###  https://bimerr.iot.linkeddata.es/def/weat#apparentTemperatureMin
<https://bimerr.iot.linkeddata.es/def/weat#apparentTemperatureMin> rdf:type owl:NamedIndividual ,
                                                                            <https://bimerr.iot.linkeddata.es/def/weat#Temperature> ;
                                                                   rdfs:comment "An individual representing the temperature property apparent temperature min from Dark Sky API." .


###  https://bimerr.iot.linkeddata.es/def/weat#apparentTemperatureMinTime
<https://bimerr.iot.linkeddata.es/def/weat#apparentTemperatureMinTime> rdf:type owl:NamedIndividual ,
                                                                                <https://bimerr.iot.linkeddata.es/def/weat#Time> ;
                                                                       rdfs:comment "An individual representing the time property apparent temperature min time from Dark Sky API." .


###  https://bimerr.iot.linkeddata.es/def/weat#cloudCover
<https://bimerr.iot.linkeddata.es/def/weat#cloudCover> rdf:type owl:NamedIndividual ,
                                                                <https://bimerr.iot.linkeddata.es/def/weat#SkyCover> ;
                                                       rdfs:comment "An individual representing the sky cover property cloud cover from Dark Sky API." .


###  https://bimerr.iot.linkeddata.es/def/weat#moonPhase
<https://bimerr.iot.linkeddata.es/def/weat#moonPhase> rdf:type owl:NamedIndividual ,
                                                               <https://bimerr.iot.linkeddata.es/def/weat#WeatherProperty> ;
                                                      rdfs:comment "An individual representing the weather property moon phase from Dark Sky API." .


###  https://bimerr.iot.linkeddata.es/def/weat#nearestStormBearing
<https://bimerr.iot.linkeddata.es/def/weat#nearestStormBearing> rdf:type owl:NamedIndividual ,
                                                                         <https://bimerr.iot.linkeddata.es/def/weat#Storm> ;
                                                                rdfs:comment "An individual representing the storm property nearest storm bearing from Dark Sky API." .


###  https://bimerr.iot.linkeddata.es/def/weat#nearestStormDistance
<https://bimerr.iot.linkeddata.es/def/weat#nearestStormDistance> rdf:type owl:NamedIndividual ,
                                                                          <https://bimerr.iot.linkeddata.es/def/weat#Storm> ;
                                                                 rdfs:comment "An individual representing the storm property nearest storm distance from Dark Sky API." .


###  https://bimerr.iot.linkeddata.es/def/weat#ozone
<https://bimerr.iot.linkeddata.es/def/weat#ozone> rdf:type owl:NamedIndividual ,
                                                           <https://bimerr.iot.linkeddata.es/def/weat#WeatherProperty> ;
                                                  rdfs:comment "An individual representing the weather property ozone from Dark Sky API." .


###  https://bimerr.iot.linkeddata.es/def/weat#precipAccumulation
<https://bimerr.iot.linkeddata.es/def/weat#precipAccumulation> rdf:type owl:NamedIndividual ,
                                                                        <https://bimerr.iot.linkeddata.es/def/weat#Precipitation> ;
                                                               rdfs:comment "An individual representing the precipitation property precipitation accumulation from Dark Sky API." .


###  https://bimerr.iot.linkeddata.es/def/weat#precipIntensity
<https://bimerr.iot.linkeddata.es/def/weat#precipIntensity> rdf:type owl:NamedIndividual ,
                                                                     <https://bimerr.iot.linkeddata.es/def/weat#Precipitation> ;
                                                            rdfs:comment "An individual representing the precipitation property precipitation intensity from Dark Sky API." .


###  https://bimerr.iot.linkeddata.es/def/weat#precipIntensityError
<https://bimerr.iot.linkeddata.es/def/weat#precipIntensityError> rdf:type owl:NamedIndividual ,
                                                                          <https://bimerr.iot.linkeddata.es/def/weat#Precipitation> ;
                                                                 rdfs:comment "An individual representing the precipitation property precipitation intensity error from Dark Sky API." .


###  https://bimerr.iot.linkeddata.es/def/weat#precipIntensityMax
<https://bimerr.iot.linkeddata.es/def/weat#precipIntensityMax> rdf:type owl:NamedIndividual ,
                                                                        <https://bimerr.iot.linkeddata.es/def/weat#Precipitation> ;
                                                               rdfs:comment "An individual representing the precipitation property precipitation intensity max from Dark Sky API." .


###  https://bimerr.iot.linkeddata.es/def/weat#precipIntensityMaxTime
<https://bimerr.iot.linkeddata.es/def/weat#precipIntensityMaxTime> rdf:type owl:NamedIndividual ,
                                                                            <https://bimerr.iot.linkeddata.es/def/weat#Time> ;
                                                                   rdfs:comment "An individual representing the time property precipitation intensity max time from Dark Sky API." .


###  https://bimerr.iot.linkeddata.es/def/weat#precipProbability
<https://bimerr.iot.linkeddata.es/def/weat#precipProbability> rdf:type owl:NamedIndividual ,
                                                                       <https://bimerr.iot.linkeddata.es/def/weat#Precipitation> ;
                                                              rdfs:comment "An individual representing the precipitation property precipitation probability from Dark Sky API." .


###  https://bimerr.iot.linkeddata.es/def/weat#precipType
<https://bimerr.iot.linkeddata.es/def/weat#precipType> rdf:type owl:NamedIndividual ,
                                                                <https://bimerr.iot.linkeddata.es/def/weat#Precipitation> ;
                                                       rdfs:comment "An individual representing the precipitation property precipitation type from Dark Sky API." .


###  https://bimerr.iot.linkeddata.es/def/weat#pressure
<https://bimerr.iot.linkeddata.es/def/weat#pressure> rdf:type owl:NamedIndividual ,
                                                              <https://bimerr.iot.linkeddata.es/def/weat#Pressure> .


###  https://bimerr.iot.linkeddata.es/def/weat#sunriseTime
<https://bimerr.iot.linkeddata.es/def/weat#sunriseTime> rdf:type owl:NamedIndividual ,
                                                                 <https://bimerr.iot.linkeddata.es/def/weat#Time> ;
                                                        rdfs:comment "An individual representing the time property sunrise time from Dark Sky API." .


###  https://bimerr.iot.linkeddata.es/def/weat#sunsetTime
<https://bimerr.iot.linkeddata.es/def/weat#sunsetTime> rdf:type owl:NamedIndividual ,
                                                                <https://bimerr.iot.linkeddata.es/def/weat#Time> ;
                                                       rdfs:comment "An individual representing the time property sunset time from Dark Sky API." .


###  https://bimerr.iot.linkeddata.es/def/weat#temperature
<https://bimerr.iot.linkeddata.es/def/weat#temperature> rdf:type owl:NamedIndividual ,
                                                                 <https://bimerr.iot.linkeddata.es/def/weat#Temperature> ;
                                                        rdfs:comment "An individual representing the temperature property temperature from Dark Sky API." .


###  https://bimerr.iot.linkeddata.es/def/weat#temperatureHigh
<https://bimerr.iot.linkeddata.es/def/weat#temperatureHigh> rdf:type owl:NamedIndividual ,
                                                                     <https://bimerr.iot.linkeddata.es/def/weat#Temperature> ;
                                                            rdfs:comment "An individual representing the temperature property temperature high from Dark Sky API." .


###  https://bimerr.iot.linkeddata.es/def/weat#temperatureHighTime
<https://bimerr.iot.linkeddata.es/def/weat#temperatureHighTime> rdf:type owl:NamedIndividual ,
                                                                         <https://bimerr.iot.linkeddata.es/def/weat#Time> ;
                                                                rdfs:comment "An individual representing the time property temperature high time from Dark Sky API." .


###  https://bimerr.iot.linkeddata.es/def/weat#temperatureLow
<https://bimerr.iot.linkeddata.es/def/weat#temperatureLow> rdf:type owl:NamedIndividual ,
                                                                    <https://bimerr.iot.linkeddata.es/def/weat#Temperature> ;
                                                           rdfs:comment "An individual representing the temperature property temperature low from Dark Sky API." .


###  https://bimerr.iot.linkeddata.es/def/weat#temperatureLowTime
<https://bimerr.iot.linkeddata.es/def/weat#temperatureLowTime> rdf:type owl:NamedIndividual ,
                                                                        <https://bimerr.iot.linkeddata.es/def/weat#Time> ;
                                                               rdfs:comment "An individual representing the time property temperature low time from Dark Sky API." .


###  https://bimerr.iot.linkeddata.es/def/weat#temperatureMax
<https://bimerr.iot.linkeddata.es/def/weat#temperatureMax> rdf:type owl:NamedIndividual ,
                                                                    <https://bimerr.iot.linkeddata.es/def/weat#Temperature> ;
                                                           rdfs:comment "An individual representing the temperature property temperature max from Dark Sky API." .


###  https://bimerr.iot.linkeddata.es/def/weat#temperatureMaxTime
<https://bimerr.iot.linkeddata.es/def/weat#temperatureMaxTime> rdf:type owl:NamedIndividual ,
                                                                        <https://bimerr.iot.linkeddata.es/def/weat#Time> ;
                                                               rdfs:comment "An individual representing the time property temperature max time from Dark Sky API." .


###  https://bimerr.iot.linkeddata.es/def/weat#temperatureMin
<https://bimerr.iot.linkeddata.es/def/weat#temperatureMin> rdf:type owl:NamedIndividual ,
                                                                    <https://bimerr.iot.linkeddata.es/def/weat#Temperature> ;
                                                           rdfs:comment "An individual representing the temperature property temperature min from Dark Sky API." .


###  https://bimerr.iot.linkeddata.es/def/weat#temperatureMinTime
<https://bimerr.iot.linkeddata.es/def/weat#temperatureMinTime> rdf:type owl:NamedIndividual ,
                                                                        <https://bimerr.iot.linkeddata.es/def/weat#Time> ;
                                                               rdfs:comment "An individual representing the time property temperature min time from Dark Sky API." .


###  https://bimerr.iot.linkeddata.es/def/weat#time
<https://bimerr.iot.linkeddata.es/def/weat#time> rdf:type owl:NamedIndividual ,
                                                          <https://bimerr.iot.linkeddata.es/def/weat#Time> ;
                                                 rdfs:comment "An individual representing the time property  time from Dark Sky API." .


###  https://bimerr.iot.linkeddata.es/def/weat#uvIndex
<https://bimerr.iot.linkeddata.es/def/weat#uvIndex> rdf:type owl:NamedIndividual ,
                                                             <https://bimerr.iot.linkeddata.es/def/weat#Radiation> ;
                                                    rdfs:comment "An individual representing the radiation property uvIndex from Dark Sky API." .


###  https://bimerr.iot.linkeddata.es/def/weat#uvIndexTime
<https://bimerr.iot.linkeddata.es/def/weat#uvIndexTime> rdf:type owl:NamedIndividual ,
                                                                 <https://bimerr.iot.linkeddata.es/def/weat#Time> ;
                                                        rdfs:comment "An individual representing the time property uv index time from Dark Sky API." .


###  https://bimerr.iot.linkeddata.es/def/weat#windBearing
<https://bimerr.iot.linkeddata.es/def/weat#windBearing> rdf:type owl:NamedIndividual ,
                                                                 <https://bimerr.iot.linkeddata.es/def/weat#Wind> ;
                                                        rdfs:comment "An individual representing the wind property wind bearing from Dark Sky API." .


###  https://bimerr.iot.linkeddata.es/def/weat#windGust
<https://bimerr.iot.linkeddata.es/def/weat#windGust> rdf:type owl:NamedIndividual ,
                                                              <https://bimerr.iot.linkeddata.es/def/weat#Wind> ;
                                                     rdfs:comment "An individual representing the wind property wind gust from Dark Sky API." .


###  https://bimerr.iot.linkeddata.es/def/weat#windGustTime
<https://bimerr.iot.linkeddata.es/def/weat#windGustTime> rdf:type owl:NamedIndividual ,
                                                                  <https://bimerr.iot.linkeddata.es/def/weat#Time> ;
                                                         rdfs:comment "An individual representing the time property wind gust time from Dark Sky API." .


###  https://bimerr.iot.linkeddata.es/def/weat#windSpeed
<https://bimerr.iot.linkeddata.es/def/weat#windSpeed> rdf:type owl:NamedIndividual ,
                                                               <https://bimerr.iot.linkeddata.es/def/weat#Wind> ;
                                                      rdfs:comment "An individual representing the wind property wind speed from EPW." .


###  Generated by the OWL API (version 5.1.9) https://github.com/owlcs/owlapi/
